checkpoint

pulse/lib/steel/pulse/Pulse.Checker.Auto.ElimPure.fst
@@ -10,12 +10,68 @@ open Pulse.Checker.Common
 open Pulse.Typing
 module Metatheory = Pulse.Typing.Metatheory
 module VP = Pulse.Checker.VPropEquiv
+module F = Pulse.Checker.Framing
 open Pulse.Reflection.Util
+
+let k_elab_unit (g:env) (ctxt:term)
+  : continuation_elaborator g ctxt g ctxt
+  = fun p r -> r
+
 let k_elab_trans (#g0 #g1 #g2:env) (#ctxt0 #ctxt1 #ctxt2:term)
                  (k0:continuation_elaborator g0 ctxt0 g1 ctxt1)
                  (k1:continuation_elaborator g1 ctxt1 g2 ctxt2 { g1 `env_extends` g0})
    : continuation_elaborator g0 ctxt0 g2 ctxt2
    = fun post_hint res -> k0 post_hint (k1 post_hint res)
+
+let vprop_equiv_typing_fwd (#g:env) (#ctxt:_) (ctxt_typing:tot_typing g ctxt Tm_VProp)
+                           (#p:_) (d:vprop_equiv g ctxt p)
+  : tot_typing g p Tm_VProp 
+  = let fwd, _ = VP.vprop_equiv_typing d in
+    fwd ctxt_typing
+
+
+let vprop_equiv_typing_bk (#g:env) (#ctxt:_) (ctxt_typing:tot_typing g ctxt Tm_VProp)
+                           (#p:_) (d:vprop_equiv g p ctxt)
+  : tot_typing g p Tm_VProp 
+  = let _, bk = VP.vprop_equiv_typing d in
+    bk ctxt_typing
+
+let k_elab_equiv (#g1 #g2:env) (#ctxt1 #ctxt1' #ctxt2 #ctxt2':term)                 
+                 (k:continuation_elaborator g1 ctxt1 g2 ctxt2)
+                 (d1:vprop_equiv g1 ctxt1 ctxt1')
+                 (d2:vprop_equiv g2 ctxt2 ctxt2')
+  : continuation_elaborator g1 ctxt1' g2 ctxt2'
+  =  fun post_hint res -> 
+        let framing_token2 : F.frame_for_req_in_ctxt g2 ctxt2 ctxt2' = 
+            let d : vprop_equiv g2 (Tm_Star ctxt2' Tm_Emp) ctxt2 = 
+              VE_Trans _ _ _ _ (VE_Comm _ _ _) (VE_Trans _ _ _ _ (VE_Unit _ _) (VE_Sym _ _ _ d2)) in
+            (| Tm_Emp, emp_typing, d |)
+        in
+        let framing_token1 : F.frame_for_req_in_ctxt g1 ctxt1' ctxt1 = 
+            let d = VE_Trans _ _ _ _ (VE_Comm _ _ _) (VE_Trans _ _ _ _ (VE_Unit _ _) d1) in
+            (| Tm_Emp, emp_typing, d |)
+        in
+        let (| st, c, st_d |) = res in
+        if not (stateful_comp c)
+        then T.fail "Unexpected non-stateful comp in continuation elaborate"
+        else (
+            let (| _, pre_typing, _, _ |) =
+                Metatheory.(st_comp_typing_inversion (comp_typing_inversion (st_typing_correctness st_d))) in
+            let (| c', st_d' |) = Pulse.Checker.Framing.apply_frame (vprop_equiv_typing_bk pre_typing d2) st_d framing_token2 in
+            let (| st, c, st_d |) = k post_hint (| st, c', st_d' |) in
+            if not (stateful_comp c)
+            then T.fail "Unexpected non-stateful comp in continuation elaborate"
+            else 
+                let (| _, pre_typing, _, _ |) =
+                    Metatheory.(st_comp_typing_inversion (comp_typing_inversion (st_typing_correctness st_d))) in
+                let (| c', st_d' |) =
+                    Pulse.Checker.Framing.apply_frame
+                        (vprop_equiv_typing_fwd pre_typing d1)
+                        st_d
+                        framing_token1 in
+                (| st, c', st_d' |)
+        )
+    
 
 let elim_pure_head =
     let elim_pure_explicit_lid = mk_steel_wrapper_lid "elim_pure_explicit" in
@@ -58,35 +114,67 @@ let elim_pure_typing (g:env) (p:host_term)
    = admit();
      T_STApp g elim_pure_head (tm_fstar (`(prop))) None (elim_pure_comp p) _ (elim_pure_head_typing g) p_prop
 
-let pure_typing_inversion (#g:env) (#p:term) (_:tot_typing g (Tm_Pure p) Tm_VProp)
-   : tot_typing g p (tm_fstar RT.tm_prop)
-   = admit()
-
+#push-options "--query_stats --fuel 2 --ifuel 2 --split_queries no --z3rlimit_factor 4"
 let elim_one_pure (#g:env) (ctxt:term) (p:term)
                   (ctxt_p_typing:tot_typing g (Tm_Star ctxt (Tm_Pure p)) Tm_VProp)
    : T.Tac (g':env { env_extends g' g } &
             tot_typing g' ctxt Tm_VProp &
             continuation_elaborator g (Tm_Star ctxt (Tm_Pure p)) g' ctxt)
    = let ctxt_typing, pure_typing = star_typing_inversion ctxt_p_typing in
-     let p_prop = pure_typing_inversion pure_typing in
+     let p_prop = Metatheory.pure_typing_inversion pure_typing in
      let v_eq = VE_Comm g ctxt (Tm_Pure p) in
-     let framing_token = 
-        (| ctxt, ctxt_typing, VE_Comm g ctxt (Tm_Pure p) |)
+     let framing_token : F.frame_for_req_in_ctxt g (Tm_Star ctxt (Tm_Pure p)) (Tm_Pure p) = 
+        (| ctxt, ctxt_typing, VE_Comm g (Tm_Pure p) ctxt  |)
      in
      match p with
      | Tm_FStar pp _ ->
-       let _ = Pulse.Checker.Framing.apply_frame ctxt_p_typing (elim_pure_typing g pp p_prop) in
+       let e1 =  (mk_elim_pure (tm_fstar pp)) in
+       let (| c1, e1_typing |) = Pulse.Checker.Framing.apply_frame ctxt_p_typing (elim_pure_typing g pp p_prop) framing_token in
+       let (| u_of_1, pre_typing, _, _ |) = Metatheory.(st_comp_typing_inversion (comp_typing_inversion (st_typing_correctness e1_typing))) in
        let x = fresh g in
-       let b = (Inl (comp_res (elim_pure_comp pp))) in
+       let b = Inl (comp_res c1) in
        let g' = extend x b g in
-       let k : continuation_elaborator g (Tm_Star ctxt (Tm_Pure p)) g' ctxt =
-           fun post_hint res -> admit()
+       let k : continuation_elaborator g (Tm_Star ctxt (Tm_Pure p)) g' (Tm_Star Tm_Emp ctxt) =
+           fun post_hint res -> 
+               let (| e2, c2, e2_typing |) = res in
+                if not (stateful_comp c2) || None? post_hint
+                then T.fail "Unexpected non-stateful comp in continuation elaborate"
+                else (
+                    let e2_typing : st_typing g' e2 c2 = e2_typing in
+                    let e2_closed = close_st_term e2 x in
+                    assume (open_st_term e2_closed x == e2);
+                    assert (comp_pre c1 == (Tm_Star ctxt (Tm_Pure p)));
+                    assert (comp_post c1 == Tm_Star Tm_Emp ctxt);
+                    assert (comp_pre c2 == Tm_Star Tm_Emp ctxt); 
+                    assume (open_term (comp_post c1) x == comp_post c1);
+                    assume (~(x `Set.mem` freevars (comp_post c2)));
+                    let Some post_hint = post_hint in
+                    if x `Set.mem` freevars post_hint.post
+                    || not (eq_tm post_hint.ret_ty (comp_res c2) &&
+                            eq_univ post_hint.u (comp_u c2) &&
+                            eq_tm post_hint.post (comp_post c2))
+                    then T.fail "Impossible"
+                    else (
+                        let pht = Pulse.Checker.Common.post_hint_typing g post_hint x in
+                        let (| e, c, e_typing |) =
+                            Pulse.Checker.Bind.mk_bind
+                                g (Tm_Star ctxt (Tm_Pure p)) 
+                                e1 e2_closed _ _ (v_as_nv x) e1_typing
+                                u_of_1 
+                                e2_typing
+                                pht.ty_typing
+                                pht.post_typing
+                        in
+                        (| e, c, e_typing |)
+                    )
+                )
 
        in
+       let k = k_elab_equiv k (VE_Refl _ _) (VE_Unit _ ctxt) in
        Pulse.Checker.Common.extends_extends_env g x b;
        (| g', Metatheory.tot_typing_weakening x b ctxt_typing, k |)
      | _ -> T.fail "unexpected pure term"
-                 
+
 let rec elim_pure_right (#g:env) (#ctxt:term) (ctxt_typing:tot_typing g ctxt Tm_VProp)
    : T.Tac (g':env { env_extends g' g } &
             ctxt':term &
@@ -99,8 +187,7 @@ let rec elim_pure_right (#g:env) (#ctxt:term) (ctxt_typing:tot_typing g ctxt Tm_
        (| g'', ctxt'', ctxt_typing'', k_elab_trans k k' |)
      | _ ->
         extends_env_refl g;
-        let k : continuation_elaborator g ctxt g ctxt = fun post_hint res -> res in
-       (| g, ctxt, ctxt_typing, k |)
+       (| g, ctxt, ctxt_typing, k_elab_unit _ _ |)
 
 module F = Pulse.Checker.Framing
 open Pulse.Checker.VPropEquiv
@@ -134,11 +221,7 @@ let rec canon_pure_right_aux (g:env) (vps:list vprop)
       let v_eq = list_as_vprop_ctx g [hd] _ _ _ (VE_Refl _ _) v_eq in
       (| hd::vps', pures, v_eq |)
 
-let vprop_equiv_typing_fwd (#g:env) (#ctxt:_) (ctxt_typing:tot_typing g ctxt Tm_VProp)
-                           (#p:_) (d:vprop_equiv g ctxt p)
-  : tot_typing g p Tm_VProp 
-  = let fwd, _ = vprop_equiv_typing d in
-    fwd ctxt_typing
+
 
 let canon_pure_right (#g:env) (#ctxt:term) (ctxt_typing:tot_typing g ctxt Tm_VProp)
   : (ctxt':term &
@@ -149,22 +232,7 @@ let canon_pure_right (#g:env) (#ctxt:term) (ctxt_typing:tot_typing g ctxt Tm_VPr
     let veq : vprop_equiv g ctxt (list_as_vprop (vps'@pures)) =
         VE_Trans _ _ _ _ (vprop_list_equiv g ctxt) veq
     in
-    let veq' :vprop_equiv g (Tm_Star (list_as_vprop (vps'@pures)) Tm_Emp) ctxt =
-        VE_Trans _ _ _ _ (VE_Comm _ _ _) (VE_Trans _ _ _ _ (VE_Unit _ _) (VE_Sym _ _ _ veq))
-    in 
-    let framing_token : Pulse.Checker.Framing.frame_for_req_in_ctxt g ctxt (list_as_vprop (vps'@pures)) = 
-        (| Tm_Emp, emp_typing, veq' |) in
-    let k : continuation_elaborator g ctxt g (list_as_vprop (vps'@pures)) =
-        fun post_hint res -> 
-            let (| st, c, st_d |) = res in
-            if not (stateful_comp c)
-            then T.fail "Unexpected non-stateful comp in continuation elaborate"
-            else (
-                let (| c', st_d' |) = Pulse.Checker.Framing.apply_frame ctxt_typing st_d framing_token in
-                (| _, _, st_d' |)
-            )
-    in
-    (| _, vprop_equiv_typing_fwd ctxt_typing veq, k |)
+    (| _, vprop_equiv_typing_fwd ctxt_typing veq, k_elab_equiv (k_elab_unit _ _) (VE_Refl _ _) veq |)
 
   
                 
@@ -177,45 +245,3 @@ let elim_pure (#g:env) (#ctxt:term) (ctxt_typing:tot_typing g ctxt Tm_VProp)
      let (| g', ctxt'', ctxt''_typing, k' |) = elim_pure_right ctxt'_typing in
      extends_env_refl g;
      (| g', ctxt'', ctxt''_typing, k_elab_trans k k' |)
-     
-
-
-
-
-// let rec maybe_add_elims
-//            (g:env)
-//            (ctxt:list term)
-//            (t:st_term)
-//   : T.Tac st_term
-//   = let wr t' = { term = t'; range = t.range } in
-//     match ctxt with
-//     | [] -> t
-//     | Tm_ExistsSL u ty b se :: rest ->
-//       let e = wr (Tm_Protect { t = wr (Tm_ElimExists { p = Tm_ExistsSL u ty b se }) }) in
-//       let x = fresh g in
-//       let px = v_as_nv x in
-//       let g = extend x (Inl ty) g in
-//       let b = open_term_nv b px in
-//       let t = maybe_add_elims g [b] t in
-//       let t = close_st_term t x in
-//       let t = Tm_Bind { binder = default_binder_annot;
-//                         head = e;
-//                         body = wr (Tm_Protect { t }) } in
-//       maybe_add_elims g rest (wr t)
-//     | Tm_Pure p :: rest ->
-//       let elim_pure_tm = 
-//         wr (Tm_STApp { head = tm_fvar (as_fv elim_pure_explicit_lid);
-//                        arg_qual = None;
-//                        arg = p })
-//       in
-//       wr (
-//         Tm_Bind { binder = default_binder_annot;
-//                   head = wr (Tm_Protect { t = elim_pure_tm } );
-//                   body = wr (Tm_Protect { t = maybe_add_elims g rest t }) }
-//       )
-
-//     | Tm_Star p q :: rest ->
-//       maybe_add_elims g (p :: q :: rest) t    
-      
-//     | _ :: rest ->
-//       maybe_add_elims g rest t
