pulse/lib/steel/pulse/Pulse.Checker.Bind.fsti
@@ -9,6 +9,30 @@ open Pulse.Elaborate.Pure
 open Pulse.Typing
 open Pulse.Checker.Common
 
+val mk_bind (g:env)
+            (pre:term)
+            (e1:st_term)
+            (e2:st_term)
+            (c1:comp_st)
+            (c2:comp_st)
+            (px:nvar)
+            (d_e1:st_typing g e1 c1)
+            (d_c1res:tot_typing g (comp_res c1) (tm_type (comp_u c1)))
+            (d_e2:st_typing (extend (snd px) (Inl (comp_res c1)) g) (open_st_term_nv e2 px) c2)
+            (res_typing:universe_of g (comp_res c2) (comp_u c2))
+            (post_typing:tot_typing (extend (snd px) (Inl (comp_res c2)) g) (open_term_nv (comp_post c2) px) Tm_VProp)
+  : T.TacH (t:st_term &
+            c:comp { stateful_comp c ==> comp_pre c == pre } &
+            st_typing g t c)
+           (requires fun _ ->
+              let _, x = px in
+              comp_pre c1 == pre /\
+              None? (lookup g x) /\
+              (~(x `Set.mem` freevars_st e2)) /\
+              open_term (comp_post c1) x == comp_pre c2 /\
+              (~ (x `Set.mem` freevars (comp_post c2))))
+           (ensures fun _ _ -> True)
+
 val check_bind (g:env)
                (t:st_term{Tm_Bind? t.term})
                (pre:term)
